more experiments with multisorted

theories_multisorted/ConcreteSyntax.v
@@ -39,20 +39,77 @@ Combined Scheme tm_vl_rect from tm_rect, vl_rect.
 (** *** Concrete renamings. *)
 (*********************************************************************************)
 
-Equations rename_ty : ren -> ty -> ty :=
-rename_ty rty (var_ty i) := var_ty (rty i) ;
-rename_ty rty (arr t1 t2) := arr (rename_ty rty t1) (rename_ty rty t2) ;
-rename_ty rty (all t) := all (rename_ty (rup rty) t).
+Fixpoint rename_ty (rty : ren) (t : ty) : ty :=
+  match t with 
+  | var_ty i => var_ty (rty i)
+  | arr t1 t2 =>arr (rename_ty rty t1) (rename_ty rty t2)
+  | all t => all (rename_ty (rup rty) t)
+  end.
 
-Equations rename_tm : ren -> ren -> tm -> tm :=
-rename_tm rty rvl (app t1 t2) := app (rename_tm rty rvl t1) (rename_tm rty rvl t2) ;
-rename_tm rty rvl (tapp t1 t2) := tapp (rename_tm rty rvl t1) (rename_ty rty t2) ;
-rename_tm rty rvl (vt v) := vt (rename_vl rty rvl v)
+Fixpoint rename_tm (rty : ren) (rvl : ren) (t : tm) : tm :=
+  match t with 
+  | app t1 t2 => app (rename_tm rty rvl t1) (rename_tm rty rvl t2)
+  | tapp t1 t2 => tapp (rename_tm rty rvl t1) (rename_ty rty t2)
+  | vt v => vt (rename_vl rty rvl v)
+  end
 
-with rename_vl : ren -> ren -> vl -> vl :=
-rename_vl rty rvl (var_vl i) := var_vl (rvl i) ;
-rename_vl rty rvl (lam t1 t2) := lam (rename_ty rty t1) (rename_tm rty (rup rvl) t2) ;
-rename_vl rty rvl (tlam t) := tlam (rename_tm (rup rty) rvl t).
+with rename_vl (rty : ren) (rvl : ren) (t : vl) : vl :=
+  match t with 
+  | var_vl i => var_vl (rvl i)
+  | lam t1 t2 => lam (rename_ty rty t1) (rename_tm rty (rup rvl) t2)
+  | tlam t => tlam (rename_tm (rup rty) rvl t)
+  end.
+
+(*********************************************************************************)
+(** *** Concrete substitutions. *)
+(*********************************************************************************)
+
+(** [subst T] represents substitutions on terms of sort [T]. *)
+Definition subst T := nat -> T.
+
+Definition scons {T} (t : T) (s : subst T) : subst T :=
+  fun i =>
+    match i with 
+    | 0 => t 
+    | S i => s i
+    end. 
+
+Definition srcomp_ty (s : subst ty) (rty : ren) : subst ty :=
+  fun i => rename_ty rty (s i).
+
+Definition srcomp_tm (s : subst tm) (rty rvl : ren) : subst tm :=
+  fun i => rename_tm rty rvl (s i).
+
+Definition srcomp_vl (s : subst vl) (rty rvl : ren) : subst vl :=
+  fun i => rename_vl rty rvl (s i).
+
+Fixpoint substitute_ty (sty : subst ty) (t : ty) : ty :=
+  match t with 
+  | var_ty i => sty i 
+  | arr t1 t2 => arr (substitute_ty sty t1) (substitute_ty sty t2)
+  | all t => 
+    let sty := scons (var_ty 0) (srcomp_ty sty rshift) in
+    all (substitute_ty sty t)
+  end.
+
+Fixpoint substitute_tm (sty : subst ty) (svl : subst vl) (t : tm) : tm :=
+  match t with 
+  | app t1 t2 => app (substitute_tm sty svl t1) (substitute_tm sty svl t2)
+  | tapp t1 t2 => tapp (substitute_tm sty svl t1) (substitute_ty sty t2) 
+  | vt v => vt (substitute_vl sty svl v)
+  end
+
+with substitute_vl (sty : subst ty) (svl : subst vl) (t : vl) : vl :=
+  match t with 
+  | var_vl i => svl i
+  | lam t1 t2 => 
+    let svl := scons (var_vl 0) (srcomp_vl svl rid rshift) in
+    lam (substitute_ty sty t1) (substitute_tm sty svl t2)
+  | tlam t => 
+    let sty := scons (var_ty 0) (srcomp_ty sty rshift) in 
+    let svl := srcomp_vl svl rshift rid in 
+    tlam (substitute_tm sty svl t)
+  end.
 
 (*********************************************************************************)
 (** *** Signature. *)
@@ -111,13 +168,90 @@ Import ConcreteSignature.
 #[local] Existing Instance sig.
 
 (*********************************************************************************)
+(** *** Custom induction principle on level one terms. *)
+(*********************************************************************************)
+
+Section CustomInd.
+  Context (P : forall m, P.expr (Kt m) -> Prop).
+  
+  Context (Hvar : forall m i, P m (P.E_var i)).
+
+  Context (Harr : forall t1 t2, P Sty t1 -> P Sty t2 -> 
+    P Sty (P.E_ctor (m := Sty) Carr (P.E_al_cons (P.E_aterm t1) (P.E_al_cons (P.E_aterm t2) P.E_al_nil)))).
+  Context (Hall : forall t, P Sty t -> 
+    P Sty (P.E_ctor (m := Sty) Call (P.E_al_cons (P.E_abind Sty (P.E_aterm t)) P.E_al_nil))).
+
+  Context (Happ : forall t1 t2, P Stm t1 -> P Stm t2 ->
+    P Stm (P.E_ctor (m := Stm) Capp (P.E_al_cons (P.E_aterm t1) (P.E_al_cons (P.E_aterm t2) P.E_al_nil)))).
+  Context (Htapp : forall t1 t2, P Stm t1 -> P Sty t2 ->
+    P Stm (P.E_ctor (m := Stm) Ctapp (P.E_al_cons (P.E_aterm t1) (P.E_al_cons (P.E_aterm t2) P.E_al_nil)))).
+  Context (Hvt : forall t, P Svl t ->
+    P Stm (P.E_ctor (m := Stm) Cvt (P.E_al_cons (P.E_aterm t) P.E_al_nil))).
+
+  Context (Hlam : forall t1 t2, P Sty t1 -> P Stm t2 ->
+    P Svl (P.E_ctor (m := Svl) Clam (P.E_al_cons (P.E_aterm t1) (P.E_al_cons (P.E_abind Svl (P.E_aterm t2)) P.E_al_nil)))).
+  Context (Htlam : forall t1, P Stm t1 ->
+    P Svl (P.E_ctor (m := Svl) Ctlam (P.E_al_cons (P.E_abind Sty (P.E_aterm t1)) P.E_al_nil))).
+  
+  Lemma custom_ind {m} : forall t : P.expr (Kt m), P m t.
+  Proof.
+  revert m. apply P.size_ind. intros m t IH. depelim m ; depelim t.
+  all: try solve [ apply Hvar ].
+  - depelim c.
+    + depelim t. depelim t1. depelim t2. depelim t2_1. depelim t2_2. 
+      apply Harr ; apply IH ; cbn ; lia.
+    + depelim t. depelim t1. depelim t2. depelim t1. 
+      apply Hall ; apply IH ; cbn ; lia.
+  - depelim c.
+    + depelim t. depelim t1. depelim t2. depelim t2_1. depelim t2_2. 
+      apply Happ ; apply IH ; cbn ; lia.
+    + depelim t. depelim t1. depelim t2. depelim t2_1. depelim t2_2. 
+      apply Htapp ; apply IH ; cbn ; lia.
+    + depelim t. depelim t1. depelim t2. 
+      apply Hvt ; apply IH ; cbn ; lia.
+  - depelim c.
+    + depelim t. depelim t1. depelim t2. depelim t2_1. depelim t2_2. depelim t2_1.
+      apply Hlam ; apply IH ; cbn ; lia.
+    + depelim t. depelim t1. depelim t2. depelim t1. 
+      apply Htlam ; apply IH ; cbn ; lia.
+  Qed. 
+
+End CustomInd.
+
+(*********************************************************************************)
 (** *** Well formed terms. *)
 (*********************************************************************************)
 
-Section Wf.
-  Context {has_var : sort -> bool}.
+(*
 
-  Inductive wf : forall {k}, P.expr k -> Prop :=
+1. Define [occurs] and [binds]. At this point we would define 
+   [has_var m := exists m', occurs m m' /\ binds m m']
+2. Sanity check: [binds m m' -> occurs m m'].
+3. [has_var m] is simply [exists m', binds m m'].
+
+*)
+
+(** [my_inv H] extends [inversion H] by running some cleanup : it simplifies
+    equations of the form [existT P x y = existT P x y'] and runs [subst]. *)
+Ltac my_inv H :=
+  inversion H ; subst ;
+  repeat match goal with 
+  | [ H' : existT _ _ _ = existT _ _ _ |- _ ] =>
+    apply inj_right_pair in H' ; subst 
+  end.
+
+Section Wf.
+  Context {has_var : sort -> SProp}.
+  Context {occurs : sort -> sort -> SProp}.
+  Context (occurs_refl : forall s, occurs s s).
+  Context (occurs_trans : forall s1 s2 s3, occurs s1 s2 -> occurs s2 s3 -> occurs s1 s3).
+  
+  (** [wf t] expresses the fact that [t] only contains variables 
+      at sorts [m] such that [has_var m]. 
+      
+      As [wf t] lives in [SProp], we don't have access to the [depelim] tactic.
+      Instead we use [my_inv]. *)
+  Inductive wf : forall {k}, P.expr k -> SProp :=
   | wf_var m i : has_var m -> wf (P.E_var (m := m) i)
   | wf_ctor m (c : ctor m) al : wf al -> wf (P.E_ctor c al)
   | wf_al_nil : wf P.E_al_nil 
@@ -126,38 +260,34 @@ Section Wf.
   | wf_abase b x : wf (P.E_abase b x)
   | wf_aterm {m} (t : P.expr (Kt m)) : wf t -> wf (P.E_aterm t)
   | wf_abind {ty} m (a : P.expr (Ka ty)) :
-    has_var m -> wf a -> wf (P.E_abind m a).
+    wf a -> wf (P.E_abind m a).
 
-  Derive Signature for wf.
-
-  #[local] Hint Constructors wf : core.
+  (** For some reason we need to re-declare the instance [EqDec (ctor m)],
+      otherwise Rocq's typeclass resolution does not pick it up. *)
+  #[local] Existing Instance ctor_EqDec.
 
   (** * Inversion lemmas. *)
 
-  Lemma wf_var_inv {m} {i} : wf (P.E_var (m := m) i) -> has_var m.
-  Proof. intros H. now depelim H. Qed.
+  Lemma wf_var_inv {m} {i} : wf (P.E_var (m := m) i) -> has_var m .
+  Proof. intros H. my_inv H ; assumption. Qed.
 
   Lemma wf_ctor_inv {m} {c : ctor m} {al} : wf (P.E_ctor c al) -> wf al.
-  Proof. intros H. now depelim H. Qed.
-
+  Proof. intros H. my_inv H ; assumption. Qed.
+  
   Lemma wf_al_cons_inv1 {ty} {tys} {a : P.expr (Ka ty)} {al : P.expr (Kal tys)} :
     wf (P.E_al_cons a al) -> wf a.
-  Proof. intros H. now depelim H. Qed.
+  Proof. intros H. my_inv H ; assumption. Qed. 
 
   Lemma wf_al_cons_inv2 {ty} {tys} {a : P.expr (Ka ty)} {al : P.expr (Kal tys)} :
     wf (P.E_al_cons a al) -> wf al.
-  Proof. intros H. now depelim H. Qed.
+  Proof. intros H. my_inv H ; assumption. Qed.
 
   Lemma wf_aterm_inv {m} {t : P.expr (Kt m)} : wf (P.E_aterm t) -> wf t.
-  Proof. intros H. now depelim H. Qed.
+  Proof. intros H. my_inv H ; assumption. Qed.
 
   Lemma wf_abind_inv {ty} {m} {a : P.expr (Ka ty)} : 
     wf (P.E_abind m a) -> wf a.
-  Proof. intros H. now depelim H. Qed.
-
-  Lemma wf_abind_inv_var {ty} {m} {a : P.expr (Ka ty)} : 
-    wf (P.E_abind m a) -> has_var m.
-  Proof. intros H. now depelim H. Qed.
+  Proof. intros H. my_inv H ; assumption. Qed.
 
   (** * Well formed renamings/substitutions. *)
 
@@ -166,48 +296,103 @@ Section Wf.
   Proof.
   #[local] Hint Extern 1 => constructor : core.
   intros H. induction t in H, r |- * ; simp rename.
-  all: solve [ depelim H ; auto ].
+  all: solve [ my_inv H ; auto ].
   Qed.
 
-  Definition wf_subst {m} (s : P.subst m) :=
+  Definition wf_subst {m} (s : P.subst m) : SProp :=
     forall i, wf (s i).
 
   Lemma wf_scons {m} (t : P.expr (Kt m)) (s : P.subst m) : 
     wf t -> wf_subst s -> wf_subst (P.scons t s).
   Proof. intros Ht Hs i. destruct i ; now cbn. Qed. 
 
-  Definition wf_vsubst (s : P.vsubst) :=
-    forall m, wf_subst (s m).
+  (** A vector of substitutions is well-formed for a given sort [mt] of terms. *)
+  Definition wf_vsubst (s : P.vsubst) (mt : sort) : SProp :=
+    forall m, has_var m -> occurs m mt -> wf_subst (s m).
 
-  Lemma wf_vsup m s : has_var m -> wf_vsubst s -> wf_vsubst (P.vsup m s).
+  Lemma wf_vsubst_occurs m m' s :
+    occurs m m' -> wf_vsubst s m' -> wf_vsubst s m.
+  Proof. 
+  intros Hm H m'' H1 H2. apply H ; try assumption. eapply occurs_trans ; eauto. 
+  Qed.  
+
+  Lemma wf_vsup m mt s : wf_vsubst s mt -> wf_vsubst (P.vsup m s) mt.
   Proof.
-  intros Hm Hs. intros m' i. unfold P.vsup. destruct (@eq_dec (@Sig.sort sig) _ m m').
+  intros Hs. intros m' Hm' Hocc i. unfold P.vsup. destruct (@eq_dec (@Sig.sort sig) _ m m').
   - subst. apply wf_scons.
     + now constructor.
-    + intros i'. unfold P.svrcomp. apply wf_rename. apply Hs.
-  - unfold P.svrcomp. apply wf_rename. apply Hs.
-  Qed.
-
-  Lemma wf_substitute {k} (s : P.vsubst) (t : P.expr k) :
-    wf_vsubst s -> wf t -> wf (P.substitute s t).
-  Proof.
-  intros Hs Ht. induction t in s, Hs, Ht |- * ; simp substitute.
-  all: try solve [ depelim Ht ; auto ].
-  - apply Hs.
-  - pose proof (Hm := wf_abind_inv_var Ht). constructor ; try assumption.
-    apply wf_abind_inv in Ht. apply IHt ; auto using wf_vsup. 
+    + intros i'. unfold P.svrcomp. apply wf_rename. now apply Hs.
+  - unfold P.svrcomp. apply wf_rename. now apply Hs.
   Qed.
 
 End Wf.
 
 (** * Specialization of [wf] to the sorts of system F. *)
 
-Definition has_var (m : sort) : bool := 
-  match m with Sty | Svl => true | Stm => false end.
+Inductive STrue : SProp := SI.
+Inductive SFalse : SProp :=.
+
+Definition has_var (m : sort) : SProp := 
+  match m with Sty | Svl => STrue | Stm => SFalse end.
  
-Definition wf0 {k} (t : P.expr k) := @wf has_var k t.
-Definition wf0_subst {m} (s : P.subst m) := @wf_subst has_var m s.
-Definition wf0_vsubst (s : P.vsubst) := @wf_vsubst has_var s.
+(* Should be reflexive and transitive. *)
+Definition occurs (m m' : sort) : SProp :=
+  match m, m' with 
+  (* Types *)
+  | Sty, Sty => STrue
+  (* Terms *) 
+  | Sty, Stm => STrue
+  | Stm, Stm => STrue
+  | Svl, Stm => STrue
+  (* Values *) 
+  | Sty, Svl => STrue
+  | Stm, Svl => STrue
+  | Svl, Svl => STrue
+  | _, _ => SFalse
+  end.
+
+Lemma occurs_refl m : occurs m m.
+Proof. now destruct m. Qed.
+
+Lemma occurs_trans m1 m2 m3 : occurs m1 m2 -> occurs m2 m3 -> occurs m1 m3.
+Proof. now destruct m1, m2, m3. Qed.
+
+Definition wf0 {k} (t : P.expr k) : SProp := @wf has_var k t.
+Definition wf0_subst {m} (s : P.subst m) : SProp := @wf_subst has_var m s.
+Definition wf0_vsubst (s : P.vsubst) (m : sort) : SProp := @wf_vsubst has_var occurs s m.
+
+Lemma wf0_substitute {m} (s : P.vsubst) (t : P.expr (Kt m)) :
+  wf0_vsubst s m -> wf0 t -> wf0 (P.substitute s t).
+Proof.
+revert s. pattern t. revert m t. apply custom_ind.
+all: intros ; cbn.
+- apply H.
+  + apply wf_var_inv in H0. assumption. 
+  + now destruct m.
+- apply wf_ctor_inv in H2. pose proof (H3 := wf_al_cons_inv1 H2).
+  apply wf_al_cons_inv2 in H2. apply wf_aterm_inv in H3.
+  apply wf_al_cons_inv1, wf_aterm_inv in H2.
+  repeat constructor.
+  + now apply H.
+  + now apply H0.
+- repeat constructor. apply H.
+  + now apply wf_vsup.
+  + admit.
+- admit.
+- admit.
+- repeat constructor. apply H.
+  + eapply wf_vsubst_occurs ; eauto using occurs_trans ; reflexivity.
+  + apply wf_ctor_inv, wf_al_cons_inv1, wf_aterm_inv in H1. assumption.
+- repeat constructor. 
+  + apply H.
+    * eapply wf_vsubst_occurs ; eauto using occurs_trans ; reflexivity.
+    * admit.
+  + apply H0.
+    * apply wf_vsup. eapply wf_vsubst_occurs ; eauto using occurs_trans ; reflexivity.
+    * admit.
+- repeat constructor. apply H.
+  + apply wf_vsup.        
+Admitted.
 
 (*********************************************************************************)
 (** *** Reification. *)
@@ -298,12 +483,6 @@ Definition eval_kind (k : kind) : Type :=
   | Kal tys => eval_arg_tys tys
   end.
 
-(*Definition eval_ctor_Sty (c : ctor Sty) : eval_arg_tys (ctor_type Sty c) -> eval_sort Sty :=
-  match c as c0 return eval_arg_tys (ctor_type Sty c0) -> eval_sort Sty with 
-  | Carr => fun '(t1, (t2, tt)) => arr t1 t2
-  | Call => fun '(t, tt) => all t
-  end.*)
-
 Definition eval_ctor (s : sort) (c : ctor s) : eval_arg_tys (ctor_type s c) -> eval_sort s :=
   match s as s0 return forall c : ctor s0, eval_arg_tys (ctor_type s0 c) -> eval_sort s0 with 
   | Sty => fun c =>
@@ -355,65 +534,6 @@ Lemma eval_reify_tm :
   (forall v (H : wf (reify_vl v)), eval (reify_vl v) H = v).
 Proof. apply tm_vl_ind. all: intros ; cbn ; f_equal ; auto using eval_reify_ty. Qed.
 
-(*
-
-Evaluation: 
-  (t' : P.expr k) -> 
-  (t : eval_kind k, H : wf0 t', eq : eval t' H = t)
-
-*)
-
-(*********************************************************************************)
-(** *** Custom induction principle on level one terms. *)
-(*********************************************************************************)
-
-Section CustomInd.
-  Context (P : forall m, P.expr (Kt m) -> Prop).
-  
-  Context (Hvar : forall m i, P m (P.E_var i)).
-
-  Context (Harr : forall t1 t2, P Sty t1 -> P Sty t2 -> 
-    P Sty (P.E_ctor (m := Sty) Carr (P.E_al_cons (P.E_aterm t1) (P.E_al_cons (P.E_aterm t2) P.E_al_nil)))).
-  Context (Hall : forall t, P Sty t -> 
-    P Sty (P.E_ctor (m := Sty) Call (P.E_al_cons (P.E_abind Sty (P.E_aterm t)) P.E_al_nil))).
-
-  Context (Happ : forall t1 t2, P Stm t1 -> P Stm t2 ->
-    P Stm (P.E_ctor (m := Stm) Capp (P.E_al_cons (P.E_aterm t1) (P.E_al_cons (P.E_aterm t2) P.E_al_nil)))).
-  Context (Htapp : forall t1 t2, P Stm t1 -> P Sty t2 ->
-    P Stm (P.E_ctor (m := Stm) Ctapp (P.E_al_cons (P.E_aterm t1) (P.E_al_cons (P.E_aterm t2) P.E_al_nil)))).
-  Context (Hvt : forall t, P Svl t ->
-    P Stm (P.E_ctor (m := Stm) Cvt (P.E_al_cons (P.E_aterm t) P.E_al_nil))).
-
-  Context (Hlam : forall t1 t2, P Sty t1 -> P Stm t2 ->
-    P Svl (P.E_ctor (m := Svl) Clam (P.E_al_cons (P.E_aterm t1) (P.E_al_cons (P.E_abind Svl (P.E_aterm t2)) P.E_al_nil)))).
-  Context (Htlam : forall t1, P Stm t1 ->
-    P Svl (P.E_ctor (m := Svl) Ctlam (P.E_al_cons (P.E_abind Sty (P.E_aterm t1)) P.E_al_nil))).
-  
-  Lemma custom_ind {m} : forall t : P.expr (Kt m), P m t.
-  Proof.
-  revert m. apply P.size_ind. intros m t IH. depelim m ; depelim t.
-  all: try solve [ apply Hvar ].
-  - depelim c.
-    + depelim t. depelim t1. depelim t2. depelim t2_1. depelim t2_2. 
-      apply Harr ; apply IH ; cbn ; lia.
-    + depelim t. depelim t1. depelim t2. depelim t1. 
-      apply Hall ; apply IH ; cbn ; lia.
-  - depelim c.
-    + depelim t. depelim t1. depelim t2. depelim t2_1. depelim t2_2. 
-      apply Happ ; apply IH ; cbn ; lia.
-    + depelim t. depelim t1. depelim t2. depelim t2_1. depelim t2_2. 
-      apply Htapp ; apply IH ; cbn ; lia.
-    + depelim t. depelim t1. depelim t2. 
-      apply Hvt ; apply IH ; cbn ; lia.
-  - depelim c.
-    + depelim t. depelim t1. depelim t2. depelim t2_1. depelim t2_2. depelim t2_1.
-      apply Hlam ; apply IH ; cbn ; lia.
-    + depelim t. depelim t1. depelim t2. depelim t1. 
-      apply Htlam ; apply IH ; cbn ; lia.
-  Qed. 
-
-End CustomInd.
-
 (*********************************************************************************)
 (** *** Transporting renamings. *)
 (*********************************************************************************)
@@ -440,36 +560,72 @@ Definition eval_rename m : eval_vren_type m -> eval_sort m -> eval_sort m :=
   | Svl => fun '(rty, rvl) t => rename_vl rty rvl t
   end.
 
-(*Lemma rename_ty_congr (r1 r2 : ren) (t1 t2 : ty) :
-  r1 =₁ r2 -> t1 = t2 -> rename_ty r1 t1 = rename_ty r2 t2.
-Proof.
-intros H <-. induction t1 in r1, r2, H |- * ; simp rename_ty. 
-- now rewrite H.
-- f_equal ; auto.
-- f_equal. apply IHt1. intros [|i] ; [reflexivity|]. cbv. now rewrite H.
-Qed.*)
-
-(*Definition wf_vren (m : sort) (r : P.vren) : Prop :=
-  match m with 
-  | Sty => r Stm =₁ rid /\ r Svl =₁ rid 
-  | Stm => r Stm =₁ rid
-  | Svl => r Stm =₁ rid
-  end.*)
-
-
 (** Push [eval] through renamings. *)
 Lemma push_eval_rename {m} (r : P.vren) (t : P.expr (Kt m)) (H : wf t) (H' : wf (P.rename r t)) : 
-   eval (P.rename r t) H' = eval_rename m (eval_vren m r) (eval t H).
+  eval (P.rename r t) H' = eval_rename m (eval_vren m r) (eval t H).
 Proof.
 revert r H H'. pattern t. revert m t. apply custom_ind.
-all: intros ; cbn in *.
-- destruct m.
-  + depelim H. depelim H'. reflexivity.
-  + depelim H.
-  + depelim H. depelim H'. reflexivity.    
-- depelim H1. cbn in H1. depelim H1. depelim H1_. depelim H1_0. depelim H1_0_1. depelim H1_0_2. cbn.
-  depelim H'. cbn in H'. depelim H'. depelim H'1. depelim H'2. depelim H'2_1. depelim H'2_2. cbn.
-  f_equal.
-  + apply H.
-  + apply H0.   
-apply H0.
+all: intros ; cbn in * ; f_equal.
+all: try solve [ apply H | apply H0 ].
+- destruct m ; cbn.
+  + reflexivity.
+  + exfalso. now apply wf_var_inv in H.
+  + reflexivity.    
+- apply (H0 (@P.vrup sig Svl r)).
+- apply (H (@P.vrup sig Sty r)).
+Qed. 
+
+(*********************************************************************************)
+(** *** Transporting substitutions. *)
+(*********************************************************************************)
+
+(** Evaluate a single substitution. *)
+Definition eval_subst {m} (s : P.subst m) (H : wf0_subst s) : subst (eval_sort m) :=
+  fun i => eval (s i) (H i).
+
+Definition eval_vsubst_type (m : sort) : Type :=
+  match m with 
+  | Sty => subst ty  
+  | Stm => subst ty * subst vl 
+  | Svl => subst ty * subst vl
+  end.
+
+(** Evaluate a vector of substitutions. *)
+Definition eval_vsubst m (s : P.vsubst) (H : wf0_vsubst s m) : eval_vsubst_type m :=
+  match m as m0 return wf0_vsubst s m0 -> eval_vsubst_type m0 with 
+  | Sty => fun H => eval_subst (s Sty) (H Sty eq_refl eq_refl)
+  | Stm => fun H => (eval_subst (s Sty) (H Sty eq_refl eq_refl), eval_subst (s Svl) (H Svl eq_refl eq_refl))
+  | Svl => fun H => (eval_subst (s Sty) (H Sty eq_refl eq_refl), eval_subst (s Svl) (H Svl eq_refl eq_refl))
+  end H.
+
+(** Evaluate [P.substitute m] into a concrete function such as [substitute_ty] or [substitute_tm]. *)
+Definition eval_substitute m : eval_vsubst_type m -> eval_sort m -> eval_sort m :=
+  match m as m0 return eval_vsubst_type m0 -> eval_sort m0 -> eval_sort m0 with 
+  | Sty => fun sty t => substitute_ty sty t
+  | Stm => fun '(sty, svl) t => substitute_tm sty svl t
+  | Svl => fun '(sty, svl) t => substitute_vl sty svl t
+  end.
+
+(** Push [eval] through substitutions. *)
+Lemma push_eval_substitute {m} (s : P.vsubst) (t : P.expr (Kt m)) 
+  (Hs : wf0_vsubst s m) (Ht : wf t) (Hst : wf0 (P.substitute s t)) :
+  eval (P.substitute s t) Hst = eval_substitute m (eval_vsubst m s Hs) (eval t Ht).
+Proof.
+revert s Hs Ht Hst. pattern t. revert m t. apply custom_ind.
+all: intros ; cbn in * ; f_equal.
+all: try solve [ apply H | apply H0 ].
+- destruct m ; cbn.
+  + cbv [eval_subst]. f_equal. admit. (* requires uip/SProp. *)
+  + exfalso. now apply wf_var_inv in Ht.
+  + cbv [eval_subst]. f_equal. admit. (* require uip/SProp. *)    
+- assert (Ht' : wf0 t). { admit. }
+  rewrite (H (@P.vsup sig Sty s) (wf_vsup Sty Sty s Hs) Ht').
+  assert (eval_subst (P.vsup Sty s Sty)
+  (wf_vsup Sty Sty s Hs Sty eq_refl eq_refl) =₁
+  scons (var_ty 0)
+  (srcomp_ty (eval_subst (s Sty) (Hs Sty eq_refl eq_refl))
+  rshift)).
+  { intros i. cbn. admit. }
+  admit.
+- setoid_rewrite (H0 s). f_equal. (* ok... *) 
+Admitted.
